Lp2lc/Active/package.lean
@@ -1,4 +1,5 @@
 
 -- STLC module exports Def and Example
 import «Lp2lc».Active.STLC.Proof
+import «Lp2lc».Active.STLC.SI.Example
 import «Lp2lc».Active.STLC.SI.Proof
